research/src/test.asp
@@ -1,0 +1,2 @@
+p(X) :- q(x).
+false :- sdf
